00Utils/Unification/Unification.thy
@@ -2,248 +2,270 @@ theory Unification
   imports Substitution
 begin        
 
+subsection \<open>Unification\<close>
+
+text \<open>Now we define the unification algorithm. It solves its constraints in the standard way (see 
+[5]), matching constructors and assembling the unifying substitution. It can only fail if it 
+encounters a constructor mismatch, or the occurs check \<open>x \<notin> uvars \<tau>\<close> fails. We must include the 
+check, despite its implications for the algorithm's time and space complexity, because without it we 
+get bogus "infinite tree" solutions and thereby lose the soundness properties of the algorithm that 
+we need for typechecking.\<close>
+
+text \<open>The unification algorithm is by far the most complicated we will encounter - most of the 
+others amount to little more than tree-walks over the relevant ASTs - and has the only really 
+interesting termination proof. We prove termination via a sequence of three measures. First, the 
+number of free variables in the constraint equations: we never add variables, and the fourth 
+recursive call eliminates at least one - note the importance of the occurs check here. Second, the
+number of constructors in the left-hand sides of the equations: the first recursive call eliminates 
+one; so does the second (the restriction to the left-hand side is precisely to ensure that this 
+call is smaller); and the third cannot increase it. Finally, the number of equations overall: this 
+decreases in the third recursive call.\<close>
+
 function unify :: "constraint \<rightharpoonup> subst" where
   "unify [] = Some Map.empty"
-| "unify ((Ctor k\<^sub>1 es\<^sub>1, Ctor k\<^sub>2 es\<^sub>2) # ess) = (
-    if k\<^sub>1 = k\<^sub>2 \<and> length es\<^sub>1 = length es\<^sub>2 then unify (zip es\<^sub>1 es\<^sub>2 @ ess)
+| "unify ((Ctor g\<^sub>1 \<tau>s\<^sub>1, Ctor g\<^sub>2 \<tau>s\<^sub>2) # \<kappa>) = (
+    if g\<^sub>1 = g\<^sub>2 \<and> length \<tau>s\<^sub>1 = length \<tau>s\<^sub>2 then unify (zip \<tau>s\<^sub>1 \<tau>s\<^sub>2 @ \<kappa>)
     else None)"
-| "unify ((Ctor k es, Var x) # ess) = unify ((Var x, Ctor k es) # ess)"
-| "unify ((Var x, e) # ess) = (
-    if e = Var x then unify ess
-    else if x \<notin> uvars e then map_option (extend_subst x e) (unify (constr_subst x e ess))
+| "unify ((Ctor g \<tau>s, Var x) # \<kappa>) = unify ((Var x, Ctor g \<tau>s) # \<kappa>)"
+| "unify ((Var x, \<tau>) # \<kappa>) = (
+    if \<tau> = Var x then unify \<kappa>
+    else if x \<notin> uvars \<tau> then map_option (extend_subst x \<tau>) (unify (constr_subst x \<tau> \<kappa>))
     else None)"
   by pat_completeness auto
 termination
   by (relation "measures [card \<circ> constr_vars, constr_ctor_count, length]") 
      (simp_all add: card_insert_if)
 
+text \<open>We prove a specialized induction principle that more closely matches the structure of the 
+algorithm, to ease proving its properties.\<close>
+
 lemma unify_induct [case_names Nil CtorCtorYes CtorCtorNo CtorVar VarSame Occurs VarNo VarYes]: "
-    P [] \<Longrightarrow>
-    (\<And>k es\<^sub>1 es\<^sub>2 ess. length es\<^sub>1 = length es\<^sub>2 \<Longrightarrow> P (zip es\<^sub>1 es\<^sub>2 @ ess) \<Longrightarrow> 
-      P ((Ctor k es\<^sub>1, Ctor k es\<^sub>2) # ess)) \<Longrightarrow>
-    (\<And>k\<^sub>1 k\<^sub>2 es\<^sub>1 es\<^sub>2 ess. k\<^sub>1 \<noteq> k\<^sub>2 \<or> length es\<^sub>1 \<noteq> length es\<^sub>2 \<Longrightarrow> 
-      P ((Ctor k\<^sub>1 es\<^sub>1, Ctor k\<^sub>2 es\<^sub>2) # ess)) \<Longrightarrow>
-    (\<And>x es k ess. P ((Var x, Ctor k es) # ess) \<Longrightarrow> P ((Ctor k es, Var x) # ess)) \<Longrightarrow>
-    (\<And>x ess. P ess \<Longrightarrow> P ((Var x, Var x) # ess)) \<Longrightarrow>
-    (\<And>x e ess. e \<noteq> Var x \<Longrightarrow> x \<in> uvars e \<Longrightarrow> P ((Var x, e) # ess)) \<Longrightarrow>
-    (\<And>x e ess. e \<noteq> Var x \<Longrightarrow> x \<notin> uvars e \<Longrightarrow> P (constr_subst x e ess) \<Longrightarrow> 
-      unify (constr_subst x e ess) = None \<Longrightarrow> P ((Var x, e) # ess)) \<Longrightarrow> 
-    (\<And>x e ess s'. e \<noteq> Var x \<Longrightarrow> x \<notin> uvars e \<Longrightarrow> P (constr_subst x e ess) \<Longrightarrow> 
-      unify (constr_subst x e ess) = Some s' \<Longrightarrow> P ((Var x, e) # ess)) \<Longrightarrow> 
-    P ts"
-proof (induction ts rule: unify.induct)
-  case (2 k\<^sub>1 es\<^sub>1 k\<^sub>2 es\<^sub>2 ess)
-  thus ?case by (cases "k\<^sub>1 = k\<^sub>2 \<and> length es\<^sub>1 = length es\<^sub>2") simp_all
+  P [] \<Longrightarrow>
+  (\<And>g \<tau>s\<^sub>1 \<tau>s\<^sub>2 \<kappa>. length \<tau>s\<^sub>1 = length \<tau>s\<^sub>2 \<Longrightarrow> P (zip \<tau>s\<^sub>1 \<tau>s\<^sub>2 @ \<kappa>) \<Longrightarrow> 
+    P ((Ctor g \<tau>s\<^sub>1, Ctor g \<tau>s\<^sub>2) # \<kappa>)) \<Longrightarrow>
+  (\<And>g\<^sub>1 g\<^sub>2 \<tau>s\<^sub>1 \<tau>s\<^sub>2 \<kappa>. g\<^sub>1 \<noteq> g\<^sub>2 \<or> length \<tau>s\<^sub>1 \<noteq> length \<tau>s\<^sub>2 \<Longrightarrow> 
+    P ((Ctor g\<^sub>1 \<tau>s\<^sub>1, Ctor g\<^sub>2 \<tau>s\<^sub>2) # \<kappa>)) \<Longrightarrow>
+  (\<And>x \<tau>s g \<kappa>. P ((Var x, Ctor g \<tau>s) # \<kappa>) \<Longrightarrow> P ((Ctor g \<tau>s, Var x) # \<kappa>)) \<Longrightarrow>
+  (\<And>x \<kappa>. P \<kappa> \<Longrightarrow> P ((Var x, Var x) # \<kappa>)) \<Longrightarrow>
+  (\<And>x \<tau> \<kappa>. \<tau> \<noteq> Var x \<Longrightarrow> x \<in> uvars \<tau> \<Longrightarrow> P ((Var x, \<tau>) # \<kappa>)) \<Longrightarrow>
+  (\<And>x \<tau> \<kappa>. \<tau> \<noteq> Var x \<Longrightarrow> x \<notin> uvars \<tau> \<Longrightarrow> P (constr_subst x \<tau> \<kappa>) \<Longrightarrow> 
+    unify (constr_subst x \<tau> \<kappa>) = None \<Longrightarrow> P ((Var x, \<tau>) # \<kappa>)) \<Longrightarrow> 
+  (\<And>x \<tau> \<kappa> \<sigma>. \<tau> \<noteq> Var x \<Longrightarrow> x \<notin> uvars \<tau> \<Longrightarrow> P (constr_subst x \<tau> \<kappa>) \<Longrightarrow> 
+    unify (constr_subst x \<tau> \<kappa>) = Some \<sigma> \<Longrightarrow> P ((Var x, \<tau>) # \<kappa>)) \<Longrightarrow> 
+  P \<kappa>"
+proof (induction \<kappa> rule: unify.induct)
+  case (2 g\<^sub>1 \<tau>s\<^sub>1 g\<^sub>2 \<tau>s\<^sub>2 \<kappa>)
+  thus ?case by (cases "g\<^sub>1 = g\<^sub>2 \<and> length \<tau>s\<^sub>1 = length \<tau>s\<^sub>2") simp_all
 next
-  case (4 x e ess)
+  case (4 x \<tau> \<kappa>)
   thus ?case 
-    by (cases "e \<noteq> Var x") (cases "x \<notin> uvars e", cases "unify (constr_subst x e ess)", simp_all)
+    by (cases "\<tau> \<noteq> Var x") (cases "x \<notin> uvars \<tau>", cases "unify (constr_subst x \<tau> \<kappa>)", simp_all)
 qed simp_all
 
-definition fail :: constraint where
-  "fail = [(Ctor ''a'' [], Ctor ''b'' [])]"
+text \<open>The domain and range of a successful substitution are limited to the variables from the 
+constraints, and are distinct from each other (and thus the substitution is idempotent).\<close>
 
-lemma unify_dom [simp]: "unify ess = Some s \<Longrightarrow> dom s \<subseteq> constr_vars ess"
-proof (induction ess arbitrary: s rule: unify_induct)
-  case (VarYes x e ess s')
-  hence "dom s' \<subseteq> constr_vars (constr_subst x e ess)" by simp
-  hence "dom (extend_subst x e s') \<subseteq> insert x (uvars e \<union> constr_vars ess)" by (auto split: if_splits)
+lemma unify_dom [simp]: "unify \<kappa> = Some \<sigma> \<Longrightarrow> dom \<sigma> \<subseteq> constr_vars \<kappa>"
+proof (induction \<kappa> arbitrary: \<sigma> rule: unify_induct)
+  case (VarYes x \<tau> \<kappa> \<sigma>')
+  hence "dom \<sigma>' \<subseteq> constr_vars (constr_subst x \<tau> \<kappa>)" by simp
+  hence "dom (extend_subst x \<tau> \<sigma>') \<subseteq> insert x (uvars \<tau> \<union> constr_vars \<kappa>)" by (auto split: if_splits)
   with VarYes show ?case by simp
 qed auto
 
-lemma unify_ran [simp]: "unify ess = Some s \<Longrightarrow> subst_vars s \<subseteq> constr_vars ess"
-proof (induction ess arbitrary: s rule: unify_induct)
-  case (VarYes x e ess s')
-  hence X: "subst_vars s' \<subseteq> constr_vars (constr_subst x e ess)" by simp
-  from VarYes have "dom s' \<subseteq> constr_vars (constr_subst x e ess)" by (metis unify_dom)
-  with VarYes have "x \<notin> dom s'" by (auto simp del: constr_subst_no_var split: if_splits)
-  hence D: "subst_vars (extend_subst x e s') = uvars (subst s' e) \<union> subst_vars s'" by simp
-  from X have "uvars e - dom s' \<union> subst_vars s' \<subseteq> insert x (uvars e \<union> constr_vars ess)" 
+lemma unify_ran [simp]: "unify \<kappa> = Some \<sigma> \<Longrightarrow> subst_vars \<sigma> \<subseteq> constr_vars \<kappa>"
+proof (induction \<kappa> arbitrary: \<sigma> rule: unify_induct)
+  case (VarYes x \<tau> \<kappa> \<sigma>')
+  hence X: "subst_vars \<sigma>' \<subseteq> constr_vars (constr_subst x \<tau> \<kappa>)" by simp
+  from VarYes have "dom \<sigma>' \<subseteq> constr_vars (constr_subst x \<tau> \<kappa>)" by (metis unify_dom)
+  with VarYes have "x \<notin> dom \<sigma>'" by (auto simp del: constr_subst_no_var split: if_splits)
+  hence D: "subst_vars (extend_subst x \<tau> \<sigma>') = uvars (subst \<sigma>' \<tau>) \<union> subst_vars \<sigma>'" by simp
+  from X have "uvars \<tau> - dom \<sigma>' \<union> subst_vars \<sigma>' \<subseteq> insert x (uvars \<tau> \<union> constr_vars \<kappa>)" 
     by (auto split: if_splits)
-  moreover have "uvars (subst s' e) \<subseteq> uvars e - dom s' \<union> subst_vars s'" by simp
-  ultimately have Y: "uvars (subst s' e) \<subseteq> insert x (uvars e \<union> constr_vars ess)" by blast
-  from X have "subst_vars s' \<subseteq> insert x (uvars e \<union> constr_vars ess)" by (auto split: if_splits)
+  moreover have "uvars (subst \<sigma>' \<tau>) \<subseteq> uvars \<tau> - dom \<sigma>' \<union> subst_vars \<sigma>'" by simp
+  ultimately have Y: "uvars (subst \<sigma>' \<tau>) \<subseteq> insert x (uvars \<tau> \<union> constr_vars \<kappa>)" by blast
+  from X have "subst_vars \<sigma>' \<subseteq> insert x (uvars \<tau> \<union> constr_vars \<kappa>)" by (auto split: if_splits)
   with VarYes D Y show ?case by simp
 qed auto
 
-lemma [simp]: "unify ess = Some s \<Longrightarrow> idempotent s"
-proof (induction ess arbitrary: s rule: unify_induct)
-  case (VarYes x e ess s')
-  hence "dom s' \<subseteq> constr_vars (constr_subst x e ess)" by (metis unify_dom)
-  hence D: "dom s' \<subseteq> constr_vars ess - {x} \<union> (if x \<in> constr_vars ess then uvars e else {})" by simp
-  from VarYes have A: "idempotent s'" by simp
-  from VarYes have B: "x \<notin> uvars e" by simp
-  from VarYes D have C: "x \<notin> dom s'" by (auto simp del: constr_subst_no_var split: if_splits)
-  from VarYes have "subst_vars s' \<subseteq> constr_vars (constr_subst x e ess)" by (metis unify_ran) 
-  with VarYes have "x \<notin> subst_vars s'" by (auto simp del: constr_subst_no_var split: if_splits)
-  with A B C have "idempotent (extend_subst x e s')" by simp
+lemma unify_idempotent [simp]: "unify \<kappa> = Some \<sigma> \<Longrightarrow> idempotent \<sigma>"
+proof (induction \<kappa> arbitrary: \<sigma> rule: unify_induct)
+  case (VarYes x \<tau> \<kappa> \<sigma>')
+  hence "dom \<sigma>' \<subseteq> constr_vars (constr_subst x \<tau> \<kappa>)" by (metis unify_dom)
+  hence D: "dom \<sigma>' \<subseteq> constr_vars \<kappa> - {x} \<union> (if x \<in> constr_vars \<kappa> then uvars \<tau> else {})" by simp
+  from VarYes have A: "idempotent \<sigma>'" by simp
+  from VarYes have B: "x \<notin> uvars \<tau>" by simp
+  from VarYes D have C: "x \<notin> dom \<sigma>'" by (auto simp del: constr_subst_no_var split: if_splits)
+  from VarYes have "subst_vars \<sigma>' \<subseteq> constr_vars (constr_subst x \<tau> \<kappa>)" by (metis unify_ran) 
+  with VarYes have "x \<notin> subst_vars \<sigma>'" by (auto simp del: constr_subst_no_var split: if_splits)
+  with A B C have "idempotent (extend_subst x \<tau> \<sigma>')" by simp
   with VarYes show ?case by simp
 qed auto
 
-lemma unify_none [simp]: "unify ess = None \<Longrightarrow> \<nexists>s'. s' unifies\<^sub>\<kappa> ess"
-proof (induction ess rule: unify_induct)
-  case (Occurs x e ess)
-  hence "\<And>s'. \<not> s' unifies Var x and e" by (metis occurs_check)
+text \<open>If unification fails, then no substitution could have succeeded:\<close>
+
+lemma unify_none [simp]: "unify \<kappa> = None \<Longrightarrow> \<nexists>\<sigma>. \<sigma> unifies\<^sub>\<kappa> \<kappa>"
+proof (induction \<kappa> rule: unify_induct)
+  case (Occurs x \<tau> \<kappa>)
+  hence "\<And>\<sigma>. \<not> \<sigma> unifies Var x and \<tau>" by (metis occurs_check)
   thus ?case by simp
 next
-  case (VarNo x e ess)
-  have "\<And>s. s unifies Var x and e \<Longrightarrow> \<not> s unifies\<^sub>\<kappa> ess" 
+  case (VarNo x \<tau> \<kappa>)
+  have "\<And>\<sigma>. \<sigma> unifies Var x and \<tau> \<Longrightarrow> \<not> \<sigma> unifies\<^sub>\<kappa> \<kappa>" 
   proof -
-    fix s
-    assume U: "s unifies Var x and e"
-    show "?thesis s" 
-    proof (cases "s x")
+    fix \<sigma>
+    assume U: "\<sigma> unifies Var x and \<tau>"
+    show "?thesis \<sigma>" 
+    proof (cases "\<sigma> x")
       case None
-      with U have "subst s e = Var x" by simp
-      with VarNo obtain y where Y: "e = Var y \<and> s y = Some (Var x)" by auto
-      with VarNo have "\<not> extend_subst x (Var y) s unifies\<^sub>\<kappa> ess" by simp
+      with U have "subst \<sigma> \<tau> = Var x" by simp
+      with VarNo obtain y where Y: "\<tau> = Var y \<and> \<sigma> y = Some (Var x)" by auto
+      with VarNo have "\<not> extend_subst x (Var y) \<sigma> unifies\<^sub>\<kappa> \<kappa>" by simp
       with None Y show ?thesis by simp
     next
       case (Some e')
-      hence S: "s(x \<mapsto> e') = s" by auto
-      from VarNo have "\<not> extend_subst x e (s(x := None)) unifies\<^sub>\<kappa> ess" by simp
+      hence S: "\<sigma>(x \<mapsto> e') = \<sigma>" by auto
+      from VarNo have "\<not> extend_subst x \<tau> (\<sigma>(x := None)) unifies\<^sub>\<kappa> \<kappa>" by simp
       with VarNo(2) U Some S show ?thesis by auto
     qed
   qed
   thus ?case by simp
 qed simp_all
- 
-lemma unify_some [simp]: "unify ess = Some s \<Longrightarrow> s unifies\<^sub>\<kappa> ess"
-  by (induction ess arbitrary: s rule: unify_induct) auto
 
-lemma [simp]: "unify ess = Some s \<Longrightarrow> t unifies\<^sub>\<kappa> ess \<Longrightarrow> idempotent t \<Longrightarrow>
-  \<exists>u. subst t = subst u \<circ> subst s \<and> idempotent u"
-proof (induction ess arbitrary: s t rule: unify_induct)
+text \<open>The most crucial property of all: if unification succeeds, then the substitution produced 
+really does unify all the constraint equations. In fact, it produces the most general unifier, in 
+that any other unifying substitution is a specialization of this one.\<close>
+ 
+lemma unify_some [simp]: "unify \<kappa> = Some \<sigma> \<Longrightarrow> \<sigma> unifies\<^sub>\<kappa> \<kappa>"
+  by (induction \<kappa> arbitrary: \<sigma> rule: unify_induct) auto
+
+lemma unify_most_general' [simp]: "unify \<kappa> = Some \<sigma> \<Longrightarrow> \<sigma>' unifies\<^sub>\<kappa> \<kappa> \<Longrightarrow> idempotent \<sigma>' \<Longrightarrow>
+  \<exists>u. subst \<sigma>' = subst u \<circ> subst \<sigma> \<and> idempotent u"
+proof (induction \<kappa> arbitrary: \<sigma> \<sigma>' rule: unify_induct)
   case Nil
   thus ?case by auto
 next
-  case (VarYes x e ess s')
-  hence "dom s' \<subseteq> constr_vars (constr_subst x e ess)" by (metis unify_dom)
-  with VarYes have D: "x \<notin> dom s'" by (auto simp del: constr_subst_no_var split: if_splits)
-  from VarYes have "subst_vars s' \<subseteq> constr_vars (constr_subst x e ess)" by (metis unify_ran)
-  with VarYes have R: "x \<notin> subst_vars s'" by (auto simp del: constr_subst_no_var split: if_splits)
+  case (VarYes x \<tau> \<kappa> \<sigma>\<^sub>1)
+  hence "dom \<sigma>\<^sub>1 \<subseteq> constr_vars (constr_subst x \<tau> \<kappa>)" by (metis unify_dom)
+  with VarYes have D: "x \<notin> dom \<sigma>\<^sub>1" by (auto simp del: constr_subst_no_var split: if_splits)
+  from VarYes have "subst_vars \<sigma>\<^sub>1 \<subseteq> constr_vars (constr_subst x \<tau> \<kappa>)" by (metis unify_ran)
+  with VarYes have R: "x \<notin> subst_vars \<sigma>\<^sub>1" by (auto simp del: constr_subst_no_var split: if_splits)
   thus ?case
-  proof (cases "t x")
+  proof (cases "\<sigma>' x")
     case None
-    with VarYes have T: "subst t e = Var x \<and> t unifies\<^sub>\<kappa> ess" by simp
-    with VarYes obtain y where Y: "e = Var y \<and> t y = Some (Var x)" by fastforce
-    with None T have "t unifies\<^sub>\<kappa> constr_subst x (Var y) ess" by simp
-    with VarYes Y obtain u where U: "subst t = subst u \<circ> subst s' \<and> idempotent u" by fastforce
-    from None have "x \<notin> dom t" by auto
-    with D U have X: "x \<notin> dom u" by (metis split_not_in_domain)
-    from T Y U have "(subst u \<circ> subst s') (Var y) = Var x" by simp
+    with VarYes have T: "subst \<sigma>' \<tau> = Var x \<and> \<sigma>' unifies\<^sub>\<kappa> \<kappa>" by simp
+    with VarYes obtain y where Y: "\<tau> = Var y \<and> \<sigma>' y = Some (Var x)" by fastforce
+    with None T have "\<sigma>' unifies\<^sub>\<kappa> constr_subst x (Var y) \<kappa>" by simp
+    with VarYes Y obtain \<sigma>\<^sub>2 where U: "subst \<sigma>' = subst \<sigma>\<^sub>2 \<circ> subst \<sigma>\<^sub>1 \<and> idempotent \<sigma>\<^sub>2" by fastforce
+    from None have "x \<notin> dom \<sigma>'" by auto
+    with D U have X: "x \<notin> dom \<sigma>\<^sub>2" by (metis split_not_in_domain)
+    from T Y U have "(subst \<sigma>\<^sub>2 \<circ> subst \<sigma>\<^sub>1) (Var y) = Var x" by simp
     thus ?thesis
     proof (induction rule: subst_subst_var)
       case Eq
       with VarYes Y show ?case by simp
     next
       case FstOnly
-      have "subst u \<circ> subst s' = subst u \<circ> subst [x \<mapsto> Var x] \<circ> subst s'" by simp
-      with D R Y U FstOnly have "subst t = subst u \<circ> subst s' \<circ> subst [x \<mapsto> e] \<and> idempotent u"
+      have "subst \<sigma>\<^sub>2 \<circ> subst \<sigma>\<^sub>1 = subst \<sigma>\<^sub>2 \<circ> subst [x \<mapsto> Var x] \<circ> subst \<sigma>\<^sub>1" by simp
+      with D R Y U FstOnly have "subst \<sigma>' = subst \<sigma>\<^sub>2 \<circ> subst \<sigma>\<^sub>1 \<circ> subst [x \<mapsto> \<tau>] \<and> idempotent \<sigma>\<^sub>2"
         using comp_assoc by blast
       with VarYes show ?case by (auto simp add: expand_extend_subst)
     next
       case SndOnly
-      with X have "subst u \<circ> subst s' = subst u \<circ> subst [y \<mapsto> Var x] \<circ> subst s'" by simp
-      hence "subst u \<circ> subst s' = subst (extend_subst y (Var x) u) \<circ> subst [x \<mapsto> Var y] \<circ> subst s'" 
+      with X have "subst \<sigma>\<^sub>2 \<circ> subst \<sigma>\<^sub>1 = subst \<sigma>\<^sub>2 \<circ> subst [y \<mapsto> Var x] \<circ> subst \<sigma>\<^sub>1" by simp
+      hence "subst \<sigma>\<^sub>2 \<circ> subst \<sigma>\<^sub>1 = subst (extend_subst y (Var x) \<sigma>\<^sub>2) \<circ> subst [x \<mapsto> Var y] \<circ> subst \<sigma>\<^sub>1" 
         by (simp add: expand_extend_subst comp_assoc)
-      with D R Y U SndOnly have S: "subst t = 
-        subst (extend_subst y (Var x) u) \<circ> subst s' \<circ> subst [x \<mapsto> e]" by (simp add: comp_assoc)
-      from SndOnly X have "u y = Some (case u x of None \<Rightarrow> Var x | Some e \<Rightarrow> e)" 
+      with D R Y U SndOnly have S: "subst \<sigma>' = 
+        subst (extend_subst y (Var x) \<sigma>\<^sub>2) \<circ> subst \<sigma>\<^sub>1 \<circ> subst [x \<mapsto> \<tau>]" by (simp add: comp_assoc)
+      from SndOnly X have "\<sigma>\<^sub>2 y = Some (case \<sigma>\<^sub>2 x of None \<Rightarrow> Var x | Some \<tau> \<Rightarrow> \<tau>)" 
         by (auto split: option.splits)
-      with VarYes U have "idempotent (extend_subst y (Var x) u)" by simp
-      moreover from VarYes S have "subst t = subst (extend_subst y (Var x) u) \<circ> subst s" 
+      with VarYes U have "idempotent (extend_subst y (Var x) \<sigma>\<^sub>2)" by simp
+      moreover from VarYes S have "subst \<sigma>' = subst (extend_subst y (Var x) \<sigma>\<^sub>2) \<circ> subst \<sigma>" 
         by (auto simp add: expand_extend_subst)
       ultimately show ?case by blast
     next
       case (Both z)
-      with X have "subst u \<circ> subst s' = subst (extend_subst x (Var z) u) \<circ> subst s'" by auto
-      hence Z: "subst u \<circ> subst s' = subst u \<circ> subst [x \<mapsto> Var z] \<circ> subst s'" 
+      with X have "subst \<sigma>\<^sub>2 \<circ> subst \<sigma>\<^sub>1 = subst (extend_subst x (Var z) \<sigma>\<^sub>2) \<circ> subst \<sigma>\<^sub>1" by auto
+      hence Z: "subst \<sigma>\<^sub>2 \<circ> subst \<sigma>\<^sub>1 = subst \<sigma>\<^sub>2 \<circ> subst [x \<mapsto> Var z] \<circ> subst \<sigma>\<^sub>1" 
         by (simp add: expand_extend_subst)
-      from D R Both have "subst s' \<circ> subst [x \<mapsto> Var y] = subst [x \<mapsto> Var z] \<circ> subst s'" by simp
-      with U Z have "subst t = subst u \<circ> subst s' \<circ> subst [x \<mapsto> Var y]" by (metis comp_assoc)
-      with Y have S: "subst t = subst u \<circ> subst s' \<circ> subst [x \<mapsto> e]" by simp
-      from U have "idempotent u" by simp
+      from D R Both have "subst \<sigma>\<^sub>1 \<circ> subst [x \<mapsto> Var y] = subst [x \<mapsto> Var z] \<circ> subst \<sigma>\<^sub>1" by simp
+      with U Z have "subst \<sigma>' = subst \<sigma>\<^sub>2 \<circ> subst \<sigma>\<^sub>1 \<circ> subst [x \<mapsto> Var y]" by (metis comp_assoc)
+      with Y have S: "subst \<sigma>' = subst \<sigma>\<^sub>2 \<circ> subst \<sigma>\<^sub>1 \<circ> subst [x \<mapsto> \<tau>]" by simp
+      from U have "idempotent \<sigma>\<^sub>2" by simp
       with VarYes S show ?case by (auto simp add: expand_extend_subst)
   qed
   next
-    case (Some e')
-    with VarYes have "e' = subst t e \<and> t unifies\<^sub>\<kappa> ess" by simp
-    with VarYes Some obtain t' where T: "t = extend_subst x e t' \<and> t' unifies\<^sub>\<kappa> constr_subst x e ess \<and> 
-      idempotent t'" by (metis dissect_subst)
-    with VarYes obtain u where "subst t' = subst u \<circ> subst s' \<and> idempotent u" by fastforce
+    case (Some \<tau>')
+    with VarYes have "\<tau>' = subst \<sigma>' \<tau> \<and> \<sigma>' unifies\<^sub>\<kappa> \<kappa>" by simp
+    with VarYes Some obtain \<sigma>\<^sub>2 where T: "\<sigma>' = extend_subst x \<tau> \<sigma>\<^sub>2 \<and> \<sigma>\<^sub>2 unifies\<^sub>\<kappa> constr_subst x \<tau> \<kappa> \<and> 
+      idempotent \<sigma>\<^sub>2" by (metis dissect_subst)
+    with VarYes obtain \<sigma>\<^sub>3 where "subst \<sigma>\<^sub>2 = subst \<sigma>\<^sub>3 \<circ> subst \<sigma>\<^sub>1 \<and> idempotent \<sigma>\<^sub>3" by fastforce
     with VarYes T show ?thesis by (auto simp add: expand_extend_subst)
   qed
 qed simp_all
 
-lemma unify_append_fst [simp]: "unify (ess\<^sub>1 @ ess\<^sub>2) = Some s \<Longrightarrow> 
-    \<exists>s\<^sub>1. unify ess\<^sub>1 = Some s\<^sub>1 \<and> s generalizes s\<^sub>1"
-  by (induction ess\<^sub>1 arbitrary: ess\<^sub>2 s rule: unify_induct) auto
-
-lemma [simp]: "unify ess\<^sub>1 = None \<Longrightarrow> unify (ess\<^sub>1 @ ess\<^sub>2) = None"
-  by (induction ess\<^sub>1 arbitrary: ess\<^sub>2 rule: unify_induct) auto
-
-lemma unify_occurs' [simp]: "e \<noteq> Var x \<Longrightarrow> x \<in> uvars e \<Longrightarrow> 
-  unify ((e', subst [x \<mapsto> e'] e) # ess) = None"
-proof (cases "unify ((e', subst [x \<mapsto> e'] e) # ess)")
-  case (Some s)
-  moreover assume "e \<noteq> Var x" and "x \<in> uvars e"
-  ultimately show ?thesis by (metis unify_some constr_unifier.simps(2) occurs_check2)
-qed simp_all
-
-lemma unify_occurs: "unify ((e, Ctor k (map (subst [x \<mapsto> e]) es)) # ess) = Some s \<Longrightarrow> x \<notin> uvarss es"
-proof 
-  assume "x \<in> uvarss es"
-  hence "unify ((e, subst [x \<mapsto> e] (Ctor k es)) # ess) = None" using unify_occurs' by fastforce
-  moreover assume "unify ((e, Ctor k (map (subst [x \<mapsto> e]) es)) # ess) = Some s"
-  ultimately show False by simp
-qed
-
-lemma [simp]: "s unifies\<^sub>\<kappa> ess \<Longrightarrow> idempotent s \<Longrightarrow> \<exists>s'. unify ess = Some s' \<and> s generalizes s'"
-proof (cases "unify ess")
+lemma unify_most_general [simp]: "\<sigma> unifies\<^sub>\<kappa> \<kappa> \<Longrightarrow> idempotent \<sigma> \<Longrightarrow> 
+  \<exists>\<sigma>'. unify \<kappa> = Some \<sigma>' \<and> \<sigma> specializes \<sigma>'"
+proof (cases "unify \<kappa>")
   case None
-  moreover assume "s unifies\<^sub>\<kappa> ess"
+  moreover assume "\<sigma> unifies\<^sub>\<kappa> \<kappa>"
   ultimately show ?thesis by (metis unify_none)
 next
-  case (Some s')
-  assume "s unifies\<^sub>\<kappa> ess" and "idempotent s"
-  with Some obtain u where "subst s = subst u \<circ> subst s' \<and> idempotent u" by fastforce
-  hence "s generalizes s'" by (auto simp add: subst_generalize_def)
+  case (Some \<sigma>')
+  assume "\<sigma> unifies\<^sub>\<kappa> \<kappa>" and "idempotent \<sigma>"
+  with Some obtain u where "subst \<sigma> = subst u \<circ> subst \<sigma>' \<and> idempotent u" by fastforce
+  hence "\<sigma> specializes \<sigma>'" by (auto simp add: subst_specialize_def)
   with Some show ?thesis by fastforce
 qed
 
-lemma [simp]: "unify (constr_subst x e' ess) = Some s \<Longrightarrow> x \<notin> uvars e' \<Longrightarrow> 
-  \<exists>s\<^sub>2. unify ess = Some s\<^sub>2 \<and> extend_subst x e' s generalizes s\<^sub>2"
+text \<open>Finally, we prove some facts about unifying appended systems of equations: if it succeeds, 
+then both halves must also succeed independently.\<close>
+
+lemma unify_append_fst [simp]: "unify (\<kappa>\<^sub>1 @ \<kappa>\<^sub>2) = Some \<sigma> \<Longrightarrow> 
+    \<exists>s\<^sub>1. unify \<kappa>\<^sub>1 = Some s\<^sub>1 \<and> \<sigma> specializes s\<^sub>1"
+  by (induction \<kappa>\<^sub>1 arbitrary: \<kappa>\<^sub>2 \<sigma> rule: unify_induct) auto
+
+lemma unify_append_none [simp]: "unify \<kappa>\<^sub>1 = None \<Longrightarrow> unify (\<kappa>\<^sub>1 @ \<kappa>\<^sub>2) = None"
+  by (induction \<kappa>\<^sub>1 arbitrary: \<kappa>\<^sub>2 rule: unify_induct) auto
+
+lemma unify_constr_subst [simp]: "unify (constr_subst x \<tau> \<kappa>) = Some \<sigma> \<Longrightarrow> x \<notin> uvars \<tau> \<Longrightarrow> 
+  \<exists>\<sigma>'. unify \<kappa> = Some \<sigma>' \<and> extend_subst x \<tau> \<sigma> specializes \<sigma>'"
 proof -
-  assume U: "unify (constr_subst x e' ess) = Some s" 
-  hence L: "s unifies\<^sub>\<kappa> constr_subst x e' ess" and O: "idempotent s" by (metis unify_some, simp)
-  assume X: "x \<notin> uvars e'"
-  hence "x \<notin> constr_vars ess - {x} \<union> (if x \<in> constr_vars ess then uvars e' else {})" by simp
-  moreover from U have "dom s \<subseteq> constr_vars (constr_subst x e' ess)" by (metis unify_dom)
-  moreover from U have "subst_vars s \<subseteq> constr_vars (constr_subst x e' ess)" by (metis unify_ran)
-  ultimately have "x \<notin> dom s" and "x \<notin> subst_vars s" by auto
+  assume U: "unify (constr_subst x \<tau> \<kappa>) = Some \<sigma>" 
+  hence L: "\<sigma> unifies\<^sub>\<kappa> constr_subst x \<tau> \<kappa>" and O: "idempotent \<sigma>" by (metis unify_some, simp)
+  assume X: "x \<notin> uvars \<tau>"
+  hence "x \<notin> constr_vars \<kappa> - {x} \<union> (if x \<in> constr_vars \<kappa> then uvars \<tau> else {})" by simp
+  moreover from U have "dom \<sigma> \<subseteq> constr_vars (constr_subst x \<tau> \<kappa>)" by (metis unify_dom)
+  moreover from U have "subst_vars \<sigma> \<subseteq> constr_vars (constr_subst x \<tau> \<kappa>)" by (metis unify_ran)
+  ultimately have "x \<notin> dom \<sigma>" and "x \<notin> subst_vars \<sigma>" by auto
   with O X L show ?thesis by simp
 qed
 
-lemma unify_append_snd [simp]: "unify (ess\<^sub>1 @ ess\<^sub>2) = Some s \<Longrightarrow> 
-    \<exists>s\<^sub>2. unify ess\<^sub>2 = Some s\<^sub>2 \<and> s generalizes s\<^sub>2"
-proof (induction ess\<^sub>1 arbitrary: ess\<^sub>2 s rule: unify_induct)
-  case (VarYes x e ess s')
-  then obtain t where T: "unify (constr_subst x e ess @ constr_subst x e ess\<^sub>2) = Some t \<and> 
-    extend_subst x e t = s" by fastforce
-  with VarYes obtain u where U: "unify (constr_subst x e ess\<^sub>2) = Some u \<and> t generalizes u" 
+lemma unify_append_snd [simp]: "unify (\<kappa>\<^sub>1 @ \<kappa>\<^sub>2) = Some \<sigma> \<Longrightarrow> 
+    \<exists>s\<^sub>2. unify \<kappa>\<^sub>2 = Some s\<^sub>2 \<and> \<sigma> specializes s\<^sub>2"
+proof (induction \<kappa>\<^sub>1 arbitrary: \<kappa>\<^sub>2 \<sigma> rule: unify_induct)
+  case (VarYes x \<tau> \<kappa> \<sigma>')
+  then obtain t where T: "unify (constr_subst x \<tau> \<kappa> @ constr_subst x \<tau> \<kappa>\<^sub>2) = Some t \<and> 
+    extend_subst x \<tau> t = \<sigma>" by fastforce
+  with VarYes obtain u where U: "unify (constr_subst x \<tau> \<kappa>\<^sub>2) = Some u \<and> t specializes u" 
     by fastforce
-  moreover with VarYes obtain s\<^sub>2 where "unify ess\<^sub>2 = Some s\<^sub>2 \<and> extend_subst x e u generalizes s\<^sub>2" 
+  moreover with VarYes obtain s\<^sub>2 where "unify \<kappa>\<^sub>2 = Some s\<^sub>2 \<and> extend_subst x \<tau> u specializes s\<^sub>2" 
     by fastforce
-  moreover with U have "extend_subst x e t generalizes extend_subst x e u" by simp
-  ultimately have "unify ess\<^sub>2 = Some s\<^sub>2 \<and> extend_subst x e t generalizes s\<^sub>2" by fastforce
+  moreover with U have "extend_subst x \<tau> t specializes extend_subst x \<tau> u" by simp
+  ultimately have "unify \<kappa>\<^sub>2 = Some s\<^sub>2 \<and> extend_subst x \<tau> t specializes s\<^sub>2" by fastforce
   with T show ?case by fastforce
 qed (simp_all split: if_splits)
 
-lemma [simp]: "unify fail = None"
+text \<open>We also define an unsatisfiable constraint. There are any number of ways of doing this; we 
+assert that \<open>a() =? b ()\<close>\<close>
+
+definition fail :: constraint where
+  "fail = [(Ctor ''a'' [], Ctor ''b'' [])]"
+
+lemma cannot_unify_fail [simp]: "unify fail = None"
   by (simp add: fail_def)
 
-lemma [simp]: "constr_vars fail = {}"
+lemma no_vars_in_fail [simp]: "constr_vars fail = {}"
   by (simp add: fail_def)
 
 end
